---
layout: intro
transition: slide-left
---

<div style="background: linear-gradient(135deg, #e0eafc 0%, #cfdef3 100%); padding: 2rem; border-radius: 12px; box-shadow: 0 2px 8px rgba(0,0,0,0.07);">

# Chapter 5: Propositional Logic

</div>

---
transition: slide-left
---

## Introduction

Propositional logic is fundamental for artificial intelligence knowledge representation, providing a precise way to encode and reason about facts. Unlike natural language, formal sentences in propositional logic support provable inference. 

<div style="background: linear-gradient(135deg, #fff5e6 0%, #ffe6cc 100%); padding: 1.5rem; border-radius: 8px; border-left: 4px solid #ff9800; margin: 1rem 0;">

**ğŸ’¡ Example:**

"If it thunders, there is lightning. There is no lightning today. Therefore, there is no thunder today." 

Logic encodes this so a computer can infer the conclusion:
- Let $T$ = "It thunders", $L$ = "There is lightning"
- Knowledge: $T â‡’ L$ and $Â¬L$
- Conclusion: $Â¬T$ (by modus tollens)

</div>

---

## Propositional Logic: The Basics

<div style="background: linear-gradient(135deg, #e3f2fd 0%, #bbdefb 100%); padding: 1.5rem; border-radius: 8px; border-left: 4px solid #2196f3; margin: 1rem 0;">

**ğŸ“˜ Definition: Logical Operators**

Sentences are assertions built from Boolean variables (True/False). The main operators:
- **Negation (Â¬):** reverses value
- **Conjunction (âˆ§):** only True if both operands are True
- **Disjunction (âˆ¨):** True if at least one operand is True
- **Implication (â‡’):** "If a, then b." False only if a is True and b is False
- **Equivalence (â‡”):** True if both operands match

</div>

---

## Propositional Logic: The Basics

<div style="background: linear-gradient(135deg, #fff5e6 0%, #ffe6cc 100%); padding: 1.5rem; border-radius: 8px; border-left: 4px solid #ff9800; margin: 1rem 0;">

**ğŸ’¡ Example:** If $a$ is "raining" and $b$ is "John is at work"
- "Either it is not raining or John is not at work" is written as $Â¬a âˆ¨ Â¬b$
- Given: "It is raining" ($a$ is True)
- Inference: "John is not at work" ($Â¬b$)

**Solution:** From $Â¬a âˆ¨ Â¬b$ and $a$, we get $Â¬b$ (by disjunctive syllogism)

</div>

---

## Truth Tables

<div style="background: linear-gradient(135deg, #e3f2fd 0%, #bbdefb 100%); padding: 1.5rem; border-radius: 8px; border-left: 4px solid #2196f3; margin: 1rem 0;">

**ğŸ“˜ Definition: Truth Tables**

Truth tables list all possible values for logical expressions.
For two variables $a$ and $b$:

| a    | b    | a âˆ§ b | a âˆ¨ b | Â¬a |  a â‡’ b |
|------|------|-------|-------|----|--------|
| True | True |  True |  True |False|  True |
| True |False | False |  True |False| False |
|False | True | False |  True |True |  True |
|False |False | False | False |True |  True |

</div>
---

## Truth Tables

<div style="background: linear-gradient(135deg, #f3e5f5 0%, #e1bee7 100%); padding: 1.5rem; border-radius: 8px; border-left: 4px solid #9c27b0; margin: 1rem 0;">

Truth table for the XOR operator ($a âŠ• b$).

**XOR is True when operands differ (one True, one False)**

| a    | b    | a âŠ• b |
|------|------|-------|
| True | True | False |
| True |False | True  |
|False | True | True  |
|False |False | False |

</div>

---

## Laws of Propositional Logic

<div style="background: linear-gradient(135deg, #e3f2fd 0%, #bbdefb 100%); padding: 1.5rem; border-radius: 8px; border-left: 4px solid #2196f3; margin: 1rem 0;">

**ğŸ“˜ Key Laws:**

- **Idempotence:** $a âˆ¨ a = a$, $a âˆ§ a = a$
- **Double Negation:** $Â¬(Â¬a) = a$
- **Commutativity/Associativity:** Order and grouping don't affect outcome
- **Distributivity:** $a âˆ§ (b âˆ¨ c) = (a âˆ§ b) âˆ¨ (a âˆ§ c)$
- **De Morgan's Laws:** $Â¬(a âˆ¨ b) = (Â¬a) âˆ§ (Â¬b)$, $Â¬(a âˆ§ b) = (Â¬a) âˆ¨ (Â¬b)$
- **Implication reduction:** $a â‡’ b = Â¬a âˆ¨ b$

</div>

---

## Laws of Propositional Logic

<div style="background: linear-gradient(135deg, #fff5e6 0%, #ffe6cc 100%); padding: 1.5rem; border-radius: 8px; border-left: 4px solid #ff9800; margin: 1rem 0;">

**ğŸ’¡ Example:** Show that $Â¬(a âˆ¨ b)$ is equivalent to $(Â¬a) âˆ§ (Â¬b)$

**Proof:** De Morgan's Law :

 **Both columns match! âœ“**

| a | b | a âˆ¨ b | Â¬(a âˆ¨ b) | Â¬a | Â¬b | (Â¬a) âˆ§ (Â¬b) |
|---|---|-------|----------|----|----|-------------|
| T | T |   T   |    F     | F  | F  |      F      |
| T | F |   T   |    F     | F  | T  |      F      |
| F | T |   T   |    F     | T  | F  |      F      |
| F | F |   F   |    T     | T  | T  |      T      |

</div>

---

## Tautologies and Satisfiability

<div style="background: linear-gradient(135deg, #e3f2fd 0%, #bbdefb 100%); padding: 1.5rem; border-radius: 8px; border-left: 4px solid #2196f3; margin: 1rem 0;">

- **Tautology:** Always True (e.g., $a âˆ¨ Â¬a$)
- **Satisfiable:** At least one assignment makes it True (e.g., $a âˆ§ b$)
- **Unsatisfiable:** No assignment makes it True (e.g., $a âˆ§ Â¬a$)
</div>

<div style="background: linear-gradient(135deg, #fff5e6 0%, #ffe6cc 100%); padding: 1.5rem; border-radius: 8px; border-left: 4px solid #ff9800; margin: 1rem 0;">

**ğŸ’¡ Example:** Prove $a âˆ¨ Â¬a$ is a tautology

Always True regardless of $a$'s value! âœ“

| a    | Â¬a   | a âˆ¨ Â¬a |
|------|------|--------|
| True | False| True   |
| False| True | True   |

</div>

---

## Tautologies and Satisfiability

<div style="background: linear-gradient(135deg, #f3e5f5 0%, #e1bee7 100%); padding: 1.5rem; border-radius: 8px; border-left: 4px solid #9c27b0; margin: 1rem 0;">

**âœï¸ Exercise:** Is $a âˆ§ b$ satisfiable?

**Solution:** Yes! When $a = True$ and $b = True$, the expression is True. Therefore, it's satisfiable (at least one assignment makes it True).

</div>

## Clauses and Canonical Forms

<div style="background: linear-gradient(135deg, #e3f2fd 0%, #bbdefb 100%); padding: 1.5rem; border-radius: 8px; border-left: 4px solid #2196f3; margin: 1rem 0;">

- **Clause:** Disjunction of literals (e.g., $a âˆ¨ Â¬b âˆ¨ c$)
- **Conjunctive Normal Form (CNF):** Conjunction of clauses: $(a âˆ¨ b) âˆ§ (c âˆ¨ Â¬d)$
- **Disjunctive Normal Form (DNF):** Disjunction of conjunctions: $(a âˆ§ b) âˆ¨ (Â¬c âˆ§ d)$

</div>

---

## Clauses and Canonical Forms

<div style="background: linear-gradient(135deg, #fff5e6 0%, #ffe6cc 100%); padding: 1.5rem; border-radius: 8px; border-left: 4px solid #ff9800; margin: 1rem 0;">

**ğŸ’¡ Example:** Convert $Â¬(a âˆ¨ b)$ to CNF

**Solution:** 
- Apply De Morgan's Law: $Â¬(a âˆ¨ b)$ â†’ $(Â¬a) âˆ§ (Â¬b)$
- This is already in CNF! (conjunction of literals)

</div>

<div style="background: linear-gradient(135deg, #f3e5f5 0%, #e1bee7 100%); padding: 1.5rem; border-radius: 8px; border-left: 4px solid #9c27b0; margin: 1rem 0;">

**âœï¸ Exercise:** Express $(a âˆ¨ b) âˆ§ (Â¬c âˆ¨ d)$ in CNF and DNF

**Solution:**
- **CNF:** $(a âˆ¨ b) âˆ§ (Â¬c âˆ¨ d)$ - Already in CNF! âœ“
- **DNF:** Using distributivity: $(a âˆ§ Â¬c) âˆ¨ (a âˆ§ d) âˆ¨ (b âˆ§ Â¬c) âˆ¨ (b âˆ§ d)$

</div>

---

## Knowledge Bases & Expert Systems

Propositional logic is the basis for knowledge-based expert systems that encode domain expertise as logical rules.  **ğŸ’¡ Example: Medical Diagnosis System** 
<div style="background: linear-gradient(135deg, #fff5e6 0%, #ffe6cc 100%); padding: 1.5rem; border-radius: 8px; border-left: 4px solid #ff9800; margin: 1rem 0;">
Patient John's symptoms:

- $c$: coughing, $t$: fever, $f$: infection, $p$: colored phlegm, $b$: bacterial infection, $a$: administer antibiotic  
**Knowledge Base:**
- $c âˆ§ t â‡’ f$ : (cough + fever â†’ infection)
- $p âˆ§ f â‡’ b$ : (colored phlegm + infection â†’ bacterial)
- $b â‡’ a$ : (bacterial infection â†’ antibiotic)

**Solution:** If John has $c = True$, $t = True$, $p = True$:
1. From $c âˆ§ t â‡’ f$: Infer $f = True$
2. From $p âˆ§ f â‡’ b$: Infer $b = True$
3. From $b â‡’ a$: Infer $a = True$ (Recommend antibiotic!)
</div>

---

## Equivalence of Expressions

<div style="background: linear-gradient(135deg, #fff5e6 0%, #ffe6cc 100%); padding: 1.5rem; border-radius: 8px; border-left: 4px solid #ff9800; margin: 1rem 0;">

**ğŸ’¡ Example:** Show $(a âˆ¨ c) âˆ§ (a âˆ¨ d) âˆ§ (b âˆ¨ c) âˆ§ (b âˆ¨ d)$ â‰¡ $(a âˆ§ b) âˆ¨ (c âˆ§ d)$

- Start: $(a âˆ¨ c) âˆ§ (a âˆ¨ d) âˆ§ (b âˆ¨ c) âˆ§ (b âˆ¨ d)$
- Group: $[(a âˆ¨ c) âˆ§ (a âˆ¨ d)] âˆ§ [(b âˆ¨ c) âˆ§ (b âˆ¨ d)]$
- Distributive: $[a âˆ¨ (c âˆ§ d)] âˆ§ [b âˆ¨ (c âˆ§ d)]$
- Distributive again: $(a âˆ§ b) âˆ¨ (c âˆ§ d)$ âœ“
</div>

**âœï¸ Exercise:** Prove $a â‡’ b$ and $Â¬b â‡’ Â¬a$ are equivalent (contraposition)
<div style="background: linear-gradient(135deg, #f3e5f5 0%, #e1bee7 100%); padding: 1.5rem; border-radius: 8px; border-left: 4px solid #9c27b0; margin: 1rem 0;">

- $a â‡’ b$ â‰¡ $Â¬a âˆ¨ b$ (implication reduction)
- $Â¬b â‡’ Â¬a$ â‰¡ $Â¬(Â¬b) âˆ¨ Â¬a$ â‰¡ $b âˆ¨ Â¬a$ (implication + double negation)
- $Â¬a âˆ¨ b$ â‰¡ $b âˆ¨ Â¬a$ (commutativity) âœ“
</div>

---

## Automated Theorem Proving Techniques

**ğŸ“˜ Key Inference Rules:**

- **Modus Ponens:** From $a â‡’ b$ and $a$, infer $b$
- **And-Elimination:** From $a âˆ§ b$, infer both $a$ and $b$
- **Or-Elimination:** From $a âˆ¨ b$ and $Â¬a$, infer $b$

<div style="background: linear-gradient(135deg, #fff5e6 0%, #ffe6cc 100%); padding: 1.5rem; border-radius: 8px; border-left: 4px solid #ff9800; margin: 1rem 0;">

- "If Alice likes daisies, she also likes roses" ($a â‡’ b$)
- "Alice likes daisies" ($a$)  
**Solution By Modus Ponens:**
- From $a â‡’ b$ and $a$, we infer $b$
- Therefore: Alice likes roses! âœ“  
**Note:** If we had $Â¬a$ instead, we couldn't infer anything about $b$ (that would be the fallacy of denying the antecedent)
</div>

---

## Proof by Contradiction & Resolution

- **Proof by Contradiction:** Assume the negation of what you want to prove and show it leads to a contradiction
- **Resolution:** Pair clauses that differ by the negation of a literal, combine to eliminate it, repeat until contradiction or end

ğŸ’¡ Example: Prove $b$ from $a â‡’ b$ and $a$

<div style="background: linear-gradient(135deg, #fff5e6 0%, #ffe6cc 100%); padding: 1.5rem; border-radius: 8px; border-left: 4px solid #ff9800; margin: 1rem 0;">

 1. Convert to CNF: $a â‡’ b$ becomes $Â¬a âˆ¨ b$
2. Knowledge Base: $\{Â¬a âˆ¨ b, a\}$
3. To prove $b$, assume $Â¬b$ (proof by contradiction)
4. New KB: $\{Â¬a âˆ¨ b, a, Â¬b\}$
5. Resolution:
   - From $Â¬a âˆ¨ b$ and $Â¬b$: get $Â¬a$
   - From $Â¬a$ and $a$: get contradiction! âŠ¥
6. Therefore $b$ must be True! âœ“

</div> 


---

## Clauses: Definite and Horn

<div style="background: linear-gradient(135deg, #e3f2fd 0%, #bbdefb 100%); padding: 1.5rem; border-radius: 8px; border-left: 4px solid #2196f3; margin: 1rem 0;">

**ğŸ“˜ Definitions:**

- **Definite Clause:** Disjunction with exactly one positive literal (e.g., $Â¬a âˆ¨ Â¬b âˆ¨ c$)
- **Horn Clause:** At most one positive literal. Useful for efficient resolution proofs

</div>

<div style="background: linear-gradient(135deg, #fff5e6 0%, #ffe6cc 100%); padding: 1.5rem; border-radius: 8px; border-left: 4px solid #ff9800; margin: 1rem 0;">

**ğŸ’¡ Example:** Convert $a âˆ§ b â‡’ c$ to Horn clause

**Solution:**
- Apply implication reduction: $a âˆ§ b â‡’ c$ â‰¡ $Â¬(a âˆ§ b) âˆ¨ c$
- Apply De Morgan's: $Â¬(a âˆ§ b) âˆ¨ c$ â‰¡ $(Â¬a âˆ¨ Â¬b) âˆ¨ c$
- Simplify: $Â¬a âˆ¨ Â¬b âˆ¨ c$ (Horn clause with 2 negative, 1 positive literal)

</div>

---

## Forward and Backward Chaining

<div style="background: linear-gradient(135deg, #e3f2fd 0%, #bbdefb 100%); padding: 1.5rem; border-radius: 8px; border-left: 4px solid #2196f3; margin: 1rem 0;">

- **Forward Chaining:** Start with known facts and use rules to infer new facts stepwise (data-driven)
- **Backward Chaining:** Start with goal, work backward to check if it can be proved (goal-driven)

</div>

<div style="background: linear-gradient(135deg, #fff5e6 0%, #ffe6cc 100%); padding: 1.5rem; border-radius: 8px; border-left: 4px solid #ff9800; margin: 1rem 0;">

**ğŸ’¡ Example: Forward Chaining**

**Rules:** $c âˆ§ t â‡’ f$, $p âˆ§ f â‡’ b$, $b â‡’ a$

**Facts:** John has $c = True$, $t = True$, $p = True$

**Solution (Forward):**
1. Apply $c âˆ§ t â‡’ f$: Since $c$ and $t$ are True â†’ infer $f = True$
2. Apply $p âˆ§ f â‡’ b$: Since $p$ and $f$ are True â†’ infer $b = True$
3. Apply $b â‡’ a$: Since $b$ is True â†’ infer $a = True$ âœ“

</div>

---

## Forward and Backward Chaining

<div style="background: linear-gradient(135deg, #e8f5e9 0%, #c8e6c9 100%); padding: 1.5rem; border-radius: 8px; border-left: 4px solid #4caf50; margin: 1rem 0;">

**ğŸ’¡ Example: Backward Chaining**


**Rules:** $c âˆ§ t â‡’ f$, $p âˆ§ f â‡’ b$, $b â‡’ a$

**Facts:** John has $c = True$, $t = True$, $p = True$

**Goal:** Prove $a = True$

1. To prove $a$, need $b$ (from $b â‡’ a$)
2. To prove $b$, need $p âˆ§ f$ (from $p âˆ§ f â‡’ b$)
3. Check $p = True$ âœ“
4. To prove $f$, need $c âˆ§ t$ (from $c âˆ§ t â‡’ f$)
5. Check $c = True$ âœ“ and $t = True$ âœ“
6. Therefore $f$, $b$, and $a$ are all True! âœ“

</div>

---

## Comparing Chaining Methods

- **Forward chaining:** May deduce many facts (some irrelevant) - Good for data-rich scenarios
- **Backward chaining:** Only deduces facts relevant to goal - More efficient in sparse KBs

**âœï¸ Exercise:** Simulate backward chaining

<div style="background: linear-gradient(135deg, #f3e5f5 0%, #e1bee7 100%); padding: 1.5rem; border-radius: 8px; border-left: 4px solid #9c27b0; margin: 1rem 0;">

**Rules:** $a âˆ§ c â‡’ q$, $d â‡’ a$, $e â‡’ c$  
**Facts:** $d = True$, $e = True$  
**Goal:** Prove $q$  
1. To prove $q$, need $a âˆ§ c$ (from $a âˆ§ c â‡’ q$)
2. To prove $a$, need $d$ (from $d â‡’ a$) â†’ Check: $d = True$ âœ“
3. Therefore $a = True$ âœ“
4. To prove $c$, need $e$ (from $e â‡’ c$) â†’ Check: $e = True$ âœ“
5. Therefore $c = True$ âœ“
6. Since both $a$ and $c$ are True â†’ $q = True$ âœ“
</div>

---

## Exercises 

<div style="background: linear-gradient(135deg, #f3e5f5 0%, #e1bee7 100%); padding: 1.5rem; border-radius: 8px; border-left: 4px solid #9c27b0; margin: 1rem 0;">

**âœï¸ Exercise 1:** Show that $a â‡’ b$ and $Â¬b â‡’ Â¬a$ are equivalent using truth tables

<!-- **Solution:**

| a | b | a â‡’ b | Â¬b | Â¬a | Â¬b â‡’ Â¬a |
|---|---|-------|----|----|---------|
| T | T |   T   | F  | F  |    T    |
| T | F |   F   | T  | F  |    F    |
| F | T |   T   | F  | T  |    T    |
| F | F |   T   | T  | T  |    T    |

Columns match! They're equivalent (contraposition) âœ“ -->

**âœï¸ Exercise 2:** Construct truth tables for XOR, NAND, NOR

<!-- **Solution:**

| a | b | XOR (a âŠ• b) | NAND (Â¬(a âˆ§ b)) | NOR (Â¬(a âˆ¨ b)) |
|---|---|-------------|-----------------|----------------|
| T | T |      F      |        F        |       F        |
| T | F |      T      |        T        |       F        |
| F | T |      T      |        T        |       F        |
| F | F |      F      |        T        |       T        | -->

**âœï¸ Exercise 3:** Forward chaining on medical KB

**KB:** $c âˆ§ t â‡’ f$, $p âˆ§ f â‡’ b$, $b â‡’ a$  
**Facts:** $c = True$, $t = True$, $p = True$

<!-- **Solution (Forward):**
1. Apply $c âˆ§ t â‡’ f$: Since $c$ and $t$ are True â†’ infer $f = True$
2. Apply $p âˆ§ f â‡’ b$: Since $p$ and $f$ are True â†’ infer $b = True$
3. Apply $b â‡’ a$: Since $b$ is True â†’ infer $a = True$ âœ“ -->

**âœï¸ Exercise 4:** Convert $Â¬(a âˆ¨ b âˆ¨ c)$ into CNF

<!-- **Solution:**
- Apply De Morgan's: $Â¬(a âˆ¨ b âˆ¨ c)$ â†’ $Â¬a âˆ§ Â¬b âˆ§ Â¬c$
- This is already in CNF! (conjunction of literals) -->


**âœï¸ Exercise 5:** Proof by contradiction: Given $a â‡’ b$ and $a$, prove $b$

<!-- 1. Assume $Â¬b$ (for contradiction).
2. From $a â‡’ b$, if $a$ is True then $b$ must be True.
3. But we assumed $Â¬b$ is True â†’ Contradiction!
4. Therefore, $b$ must be True. -->

</div>

